MPPA - Added optim for long unsigned cmp to 0.

mppa_k1c/TargetPrinter.ml
@@ -252,7 +252,7 @@ module Target : TARGET =
          fprintf oc "	compw.%a	%a = %a, %a\n;;\n" icond it ireg rd ireg rs1 ireg rs2
       | Pcompd (it, rd, rs1, rs2) ->
          fprintf oc "	compd.%a	%a = %a, %a\n;;\n" icond it ireg rd ireg rs1 ireg rs2
-      | Pcb (bt, r, lbl) ->
+      | Pcb (bt, r, lbl) | Pcbu (bt, r, lbl) ->
          fprintf oc "	cb.%a	%a?%a\n;;\n" bcond bt ireg r print_label lbl
 
       | Plb(rd, ra, ofs) ->
